\documentclass[a4j,twocolumn,10pt,fleqn]{jarticle}
\usepackage[dvipdfmx]{graphicx}
% \usepackage[dvipdfmx]{color}
\usepackage{here}
\usepackage{longtable}
\usepackage{bm}
\usepackage{amsmath,amssymb}
\usepackage{float}
\usepackage{txfonts}
\usepackage{mathrsfs}
\usepackage{subcaption}
\usepackage{lscape}
\usepackage{textcomp}
\usepackage{multirow}
\usepackage{afterpage}
\usepackage{color}
\usepackage{tabularx}
\usepackage{pythontex}
\begin{document}
tip: $ax^2 + bx + c$\\ 
~~~~~~~~~$= a(x^2 + \frac{b}{a}x) + c$\\ 
~~~~~~~~~$= a(x + \frac{b}{2a})^2 - \left(\frac{b}{2a}\right)^2+ c$\\ 
~~~~~~~~~$= a(x + p)^2 + q$


(1)~~$4x^2-8x +6$

~~~~~~~~~$=4(x^2-2x) +6$

~~~~~~~~~$=4(x-1)^2-4+6$

~~~~~~~~~$=4(x-1)^2 +2$

(2)~~$-3x^2 +30x-80$

~~~~~~~~~$=-3(x^2-10x)-80$

~~~~~~~~~$=-3(x-5)^2 +75-80$

~~~~~~~~~$=-3(x-5)^2-5$

(3)~~$-3x^2 +6x-2$

~~~~~~~~~$=-3(x^2-2x)-2$

~~~~~~~~~$=-3(x-1)^2 +3-2$

~~~~~~~~~$=-3(x-1)^2 +1$

(4)~~$3x^2-36x +107$

~~~~~~~~~$=3(x^2-12x) +107$

~~~~~~~~~$=3(x-6)^2-108+107$

~~~~~~~~~$=3(x-6)^2-1$

(5)~~$4x^2-16x +19$

~~~~~~~~~$=4(x^2-4x) +19$

~~~~~~~~~$=4(x-2)^2-16+19$

~~~~~~~~~$=4(x-2)^2 +3$

(6)~~$-2x^2-16x-29$

~~~~~~~~~$=-2(x^2 +8x)-29$

~~~~~~~~~$=-2(x +4)^2 +32-29$

~~~~~~~~~$=-2(x +4)^2 +3$

(7)~~$-4x^2-24x-38$

~~~~~~~~~$=-4(x^2 +6x)-38$

~~~~~~~~~$=-4(x +3)^2 +36-38$

~~~~~~~~~$=-4(x +3)^2-2$

(8)~~$-4x^2 +24x-34$

~~~~~~~~~$=-4(x^2-6x)-34$

~~~~~~~~~$=-4(x-3)^2 +36-34$

~~~~~~~~~$=-4(x-3)^2 +2$

(9)~~$4x^2-40x +101$

~~~~~~~~~$=4(x^2-10x) +101$

~~~~~~~~~$=4(x-5)^2-100+101$

~~~~~~~~~$=4(x-5)^2 +1$

(10)~~$3x^2 +36x +107$

~~~~~~~~~$=3(x^2 +12x) +107$

~~~~~~~~~$=3(x +6)^2-108+107$

~~~~~~~~~$=3(x +6)^2-1$

(11)~~$3x^2-18x +22$

~~~~~~~~~$=3(x^2-6x) +22$

~~~~~~~~~$=3(x-3)^2-27+22$

~~~~~~~~~$=3(x-3)^2-5$

(12)~~$-2x^2-20x-52$

~~~~~~~~~$=-2(x^2 +10x)-52$

~~~~~~~~~$=-2(x +5)^2 +50-52$

~~~~~~~~~$=-2(x +5)^2-2$

(13)~~$-2x^2-12x-21$

~~~~~~~~~$=-2(x^2 +6x)-21$

~~~~~~~~~$=-2(x +3)^2 +18-21$

~~~~~~~~~$=-2(x +3)^2-3$

(14)~~$4x^2 +56x +197$

~~~~~~~~~$=4(x^2 +14x) +197$

~~~~~~~~~$=4(x +7)^2-196+197$

~~~~~~~~~$=4(x +7)^2 +1$

(15)~~$-x^2 +20x-103$

~~~~~~~~~$=-(x^2-20x)-103$

~~~~~~~~~$=-(x-10)^2 +100-103$

~~~~~~~~~$=-(x-10)^2-3$

(16)~~$x^2-2x +2$

~~~~~~~~~$=(x-1)^2 -1+2$

~~~~~~~~~$=(x-1)^2 +1$

(17)~~$x^2 +16x +60$

~~~~~~~~~$=(x +8)^2 -64+60$

~~~~~~~~~$=(x +8)^2-4$

(18)~~$3x^2-24x +45$

~~~~~~~~~$=3(x^2-8x) +45$

~~~~~~~~~$=3(x-4)^2-48+45$

~~~~~~~~~$=3(x-4)^2-3$

(19)~~$-2x^2-32x-129$

~~~~~~~~~$=-2(x^2 +16x)-129$

~~~~~~~~~$=-2(x +8)^2 +128-129$

~~~~~~~~~$=-2(x +8)^2-1$

(20)~~$-x^2 +18x-82$

~~~~~~~~~$=-(x^2-18x)-82$

~~~~~~~~~$=-(x-9)^2 +81-82$

~~~~~~~~~$=-(x-9)^2-1$

(21)~~$4x^2-56x +193$

~~~~~~~~~$=4(x^2-14x) +193$

~~~~~~~~~$=4(x-7)^2-196+193$

~~~~~~~~~$=4(x-7)^2-3$

(22)~~$4x^2-8x +1$

~~~~~~~~~$=4(x^2-2x) +1$

~~~~~~~~~$=4(x-1)^2-4+1$

~~~~~~~~~$=4(x-1)^2-3$

(23)~~$-5x^2 +100x-497$

~~~~~~~~~$=-5(x^2-20x)-497$

~~~~~~~~~$=-5(x-10)^2 +500-497$

~~~~~~~~~$=-5(x-10)^2 +3$

(24)~~$-3x^2 +36x-111$

~~~~~~~~~$=-3(x^2-12x)-111$

~~~~~~~~~$=-3(x-6)^2 +108-111$

~~~~~~~~~$=-3(x-6)^2-3$

(25)~~$-4x^2 +16x-20$

~~~~~~~~~$=-4(x^2-4x)-20$

~~~~~~~~~$=-4(x-2)^2 +16-20$

~~~~~~~~~$=-4(x-2)^2-4$

(26)~~$2x^2 +28x +100$

~~~~~~~~~$=2(x^2 +14x) +100$

~~~~~~~~~$=2(x +7)^2-98+100$

~~~~~~~~~$=2(x +7)^2 +2$

(27)~~$4x^2-40x +96$

~~~~~~~~~$=4(x^2-10x) +96$

~~~~~~~~~$=4(x-5)^2-100+96$

~~~~~~~~~$=4(x-5)^2-4$

(28)~~$4x^2 +24x +35$

~~~~~~~~~$=4(x^2 +6x) +35$

~~~~~~~~~$=4(x +3)^2-36+35$

~~~~~~~~~$=4(x +3)^2-1$

(29)~~$-4x^2 +72x-329$

~~~~~~~~~$=-4(x^2-18x)-329$

~~~~~~~~~$=-4(x-9)^2 +324-329$

~~~~~~~~~$=-4(x-9)^2-5$

(30)~~$-x^2 +4x-5$

~~~~~~~~~$=-(x^2-4x)-5$

~~~~~~~~~$=-(x-2)^2 +4-5$

~~~~~~~~~$=-(x-2)^2-1$

(31)~~$-5x^2 +30x-41$

~~~~~~~~~$=-5(x^2-6x)-41$

~~~~~~~~~$=-5(x-3)^2 +45-41$

~~~~~~~~~$=-5(x-3)^2 +4$

(32)~~$-5x^2 +60x-182$

~~~~~~~~~$=-5(x^2-12x)-182$

~~~~~~~~~$=-5(x-6)^2 +180-182$

~~~~~~~~~$=-5(x-6)^2-2$

(33)~~$4x^2 +8x +7$

~~~~~~~~~$=4(x^2 +2x) +7$

~~~~~~~~~$=4(x +1)^2-4+7$

~~~~~~~~~$=4(x +1)^2 +3$

(34)~~$x^2-2x +5$

~~~~~~~~~$=(x-1)^2 -1+5$

~~~~~~~~~$=(x-1)^2 +4$

(35)~~$-4x^2 +64x-254$

~~~~~~~~~$=-4(x^2-16x)-254$

~~~~~~~~~$=-4(x-8)^2 +256-254$

~~~~~~~~~$=-4(x-8)^2 +2$

(36)~~$-x^2-8x-20$

~~~~~~~~~$=-(x^2 +8x)-20$

~~~~~~~~~$=-(x +4)^2 +16-20$

~~~~~~~~~$=-(x +4)^2-4$

(37)~~$-3x^2 +6x-8$

~~~~~~~~~$=-3(x^2-2x)-8$

~~~~~~~~~$=-3(x-1)^2 +3-8$

~~~~~~~~~$=-3(x-1)^2-5$

(38)~~$-2x^2 +24x-74$

~~~~~~~~~$=-2(x^2-12x)-74$

~~~~~~~~~$=-2(x-6)^2 +72-74$

~~~~~~~~~$=-2(x-6)^2-2$

(39)~~$3x^2-24x +46$

~~~~~~~~~$=3(x^2-8x) +46$

~~~~~~~~~$=3(x-4)^2-48+46$

~~~~~~~~~$=3(x-4)^2-2$

(40)~~$-x^2 +16x-63$

~~~~~~~~~$=-(x^2-16x)-63$

~~~~~~~~~$=-(x-8)^2 +64-63$

~~~~~~~~~$=-(x-8)^2 +1$

(41)~~$-4x^2-24x-40$

~~~~~~~~~$=-4(x^2 +6x)-40$

~~~~~~~~~$=-4(x +3)^2 +36-40$

~~~~~~~~~$=-4(x +3)^2-4$

(42)~~$x^2 +10x +28$

~~~~~~~~~$=(x +5)^2 -25+28$

~~~~~~~~~$=(x +5)^2 +3$

(43)~~$-3x^2-30x-72$

~~~~~~~~~$=-3(x^2 +10x)-72$

~~~~~~~~~$=-3(x +5)^2 +75-72$

~~~~~~~~~$=-3(x +5)^2 +3$

(44)~~$4x^2 +8x$

~~~~~~~~~$=4(x^2 +2x)$

~~~~~~~~~$=4(x +1)^2-4$

(45)~~$-x^2 +18x-83$

~~~~~~~~~$=-(x^2-18x)-83$

~~~~~~~~~$=-(x-9)^2 +81-83$

~~~~~~~~~$=-(x-9)^2-2$

(46)~~$x^2-12x +38$

~~~~~~~~~$=(x-6)^2 -36+38$

~~~~~~~~~$=(x-6)^2 +2$

(47)~~$2x^2-4x-3$

~~~~~~~~~$=2(x^2-2x)-3$

~~~~~~~~~$=2(x-1)^2-2-3$

~~~~~~~~~$=2(x-1)^2-5$

(48)~~$x^2 +14x +53$

~~~~~~~~~$=(x +7)^2 -49+53$

~~~~~~~~~$=(x +7)^2 +4$

(49)~~$-2x^2 +24x-68$

~~~~~~~~~$=-2(x^2-12x)-68$

~~~~~~~~~$=-2(x-6)^2 +72-68$

~~~~~~~~~$=-2(x-6)^2 +4$

(50)~~$-5x^2 +20x-21$

~~~~~~~~~$=-5(x^2-4x)-21$

~~~~~~~~~$=-5(x-2)^2 +20-21$

~~~~~~~~~$=-5(x-2)^2-1$

\end{document}
