\documentclass[a4j,twocolumn,10pt,fleqn]{jarticle}
\usepackage[dvipdfmx]{graphicx}
% \usepackage[dvipdfmx]{color}
\usepackage{here}
\usepackage{longtable}
\usepackage{bm}
\usepackage{amsmath,amssymb}
\usepackage{float}
\usepackage{txfonts}
\usepackage{mathrsfs}
\usepackage{subcaption}
\usepackage{lscape}
\usepackage{textcomp}
\usepackage{multirow}
\usepackage{afterpage}
\usepackage{color}
\usepackage{tabularx}
\usepackage{pythontex}
\begin{document}
tip1: $\left(a x + b\right)^{3}$

~~~~~~~~~$=a^{3} x^{3} + 3 a^{2} b x^{2} + 3 a b^{2} x + b^{3}$


tip2: $\left(a x - b\right)^{3}$

~~~~~~~~~$=a^{3} x^{3} - 3 a^{2} b x^{2} + 3 a b^{2} x - b^{3}$


(1)~~$2\left(x + 2\right)^{3}$

~~~~~~~~~$=2(x^{3} + 6 x^{2} + 12 x + 8)$

~~~~~~~~~$=2 x^{3} + 12 x^{2} + 24 x + 16$

(2)~~$\left(3 x - 4\right)^{3}$

~~~~~~~~~$=27 x^{3} - 108 x^{2} + 144 x - 64$

(3)~~$-\left(5 x + 8\right)^{3}$

~~~~~~~~~$=-(125 x^{3} + 600 x^{2} + 960 x + 512)$

~~~~~~~~~$=- 125 x^{3} - 600 x^{2} - 960 x - 512$

(4)~~$-\left(2 x - 1\right)^{3}$

~~~~~~~~~$=-(8 x^{3} - 12 x^{2} + 6 x - 1)$

~~~~~~~~~$=- 8 x^{3} + 12 x^{2} - 6 x + 1$

(5)~~$-\left(4 x + 3\right)^{3}$

~~~~~~~~~$=-(64 x^{3} + 144 x^{2} + 108 x + 27)$

~~~~~~~~~$=- 64 x^{3} - 144 x^{2} - 108 x - 27$

(6)~~$-\left(5 x + 1\right)^{3}$

~~~~~~~~~$=-(125 x^{3} + 75 x^{2} + 15 x + 1)$

~~~~~~~~~$=- 125 x^{3} - 75 x^{2} - 15 x - 1$

(7)~~$\left(x + 8\right)^{3}$

~~~~~~~~~$=x^{3} + 24 x^{2} + 192 x + 512$

(8)~~$-\left(x - 1\right)^{3}$

~~~~~~~~~$=-(x^{3} - 3 x^{2} + 3 x - 1)$

~~~~~~~~~$=- x^{3} + 3 x^{2} - 3 x + 1$

(9)~~$-\left(5 x + 7\right)^{3}$

~~~~~~~~~$=-(125 x^{3} + 525 x^{2} + 735 x + 343)$

~~~~~~~~~$=- 125 x^{3} - 525 x^{2} - 735 x - 343$

(10)~~$-\left(x - 2\right)^{3}$

~~~~~~~~~$=-(x^{3} - 6 x^{2} + 12 x - 8)$

~~~~~~~~~$=- x^{3} + 6 x^{2} - 12 x + 8$

(11)~~$\left(x - 2\right)^{3}$

~~~~~~~~~$=x^{3} - 6 x^{2} + 12 x - 8$

(12)~~$-2\left(x - 3\right)^{3}$

~~~~~~~~~$=-2(x^{3} - 9 x^{2} + 27 x - 27)$

~~~~~~~~~$=- 2 x^{3} + 18 x^{2} - 54 x + 54$

(13)~~$\left(x + 1\right)^{3}$

~~~~~~~~~$=x^{3} + 3 x^{2} + 3 x + 1$

(14)~~$-\left(x + 4\right)^{3}$

~~~~~~~~~$=-(x^{3} + 12 x^{2} + 48 x + 64)$

~~~~~~~~~$=- x^{3} - 12 x^{2} - 48 x - 64$

(15)~~$-\left(x - 3\right)^{3}$

~~~~~~~~~$=-(x^{3} - 9 x^{2} + 27 x - 27)$

~~~~~~~~~$=- x^{3} + 9 x^{2} - 27 x + 27$

(16)~~$2\left(x + 3\right)^{3}$

~~~~~~~~~$=2(x^{3} + 9 x^{2} + 27 x + 27)$

~~~~~~~~~$=2 x^{3} + 18 x^{2} + 54 x + 54$

(17)~~$-\left(x + 6\right)^{3}$

~~~~~~~~~$=-(x^{3} + 18 x^{2} + 108 x + 216)$

~~~~~~~~~$=- x^{3} - 18 x^{2} - 108 x - 216$

(18)~~$-\left(x - 4\right)^{3}$

~~~~~~~~~$=-(x^{3} - 12 x^{2} + 48 x - 64)$

~~~~~~~~~$=- x^{3} + 12 x^{2} - 48 x + 64$

(19)~~$-\left(3 x - 8\right)^{3}$

~~~~~~~~~$=-(27 x^{3} - 216 x^{2} + 576 x - 512)$

~~~~~~~~~$=- 27 x^{3} + 216 x^{2} - 576 x + 512$

(20)~~$\left(3 x + 7\right)^{3}$

~~~~~~~~~$=27 x^{3} + 189 x^{2} + 441 x + 343$

\end{document}
