\documentclass[a4j,twocolumn,10pt,fleqn]{jarticle}
\usepackage[dvipdfmx]{graphicx}
% \usepackage[dvipdfmx]{color}
\usepackage{here}
\usepackage{longtable}
\usepackage{bm}
\usepackage{amsmath,amssymb}
\usepackage{float}
\usepackage{txfonts}
\usepackage{mathrsfs}
\usepackage{subcaption}
\usepackage{lscape}
\usepackage{textcomp}
\usepackage{multirow}
\usepackage{afterpage}
\usepackage{color}
\usepackage{tabularx}
\usepackage{pythontex}
\begin{document}
tip:~~$Pacx^2 + P(ad + bc)x + Pbd$

~~~~~~~~~$= P\{acx^2 + (ad + bc)x +bd\}$

~~~~~~~~~$= P(ax + b)(cx + d)$

(1)~~$-20x^2~-85x~-90$

~~~~~~~~~$=-5(4x^2~+~17x~+~18)$

~~~~~~~~~$=-5(4x+9)(x+2)$

(2)~~$-15x^2~-2x~+~1$

~~~~~~~~~$=-(15x^2~+~2x~-1)$

~~~~~~~~~$=-(3x+1)(5x-1)$

(3)~~$4x^2~-26x~-48$

~~~~~~~~~$=2(2x^2~-13x~-24)$

~~~~~~~~~$=2(2x+3)(x-8)$

(4)~~$-16x^2~-24x~+~27$

~~~~~~~~~$=-(16x^2~+~24x~-27)$

~~~~~~~~~$=-(4x-3)(4x+9)$

(5)~~$-15x^2~+~2x~+~45$

~~~~~~~~~$=-(15x^2~-2x~-45)$

~~~~~~~~~$=-(3x+5)(5x-9)$

(6)~~$12x^2~+~27x$

~~~~~~~~~$=3x(4x+9)$

(7)~~$-2x^2~+~10x$

~~~~~~~~~$=-2x(x-5)$

(8)~~$-8x^2~-18x~+~35$

~~~~~~~~~$=-(8x^2~+~18x~-35)$

~~~~~~~~~$=-(2x+7)(4x-5)$

(9)~~$12x^2~+~5x~-28$

~~~~~~~~~$=(3x-4)(4x+7)$

(10)~~$-5x^2~-32x~-12$

~~~~~~~~~$=-(5x^2~+~32x~+~12)$

~~~~~~~~~$=-(5x+2)(x+6)$

(11)~~$6x^2~+~2x~-48$

~~~~~~~~~$=2(3x^2~+~x~-24)$

~~~~~~~~~$=2(3x-8)(x+3)$

(12)~~$-8x~-8$

~~~~~~~~~$=-8(x+1)$

(13)~~$6x^2~-35x~+~36$

~~~~~~~~~$=(2x-9)(3x-4)$

(14)~~$-16x^2~+~4x~+~2$

~~~~~~~~~$=-2(8x^2~-2x~-1)$

~~~~~~~~~$=-2(4x+1)(2x-1)$

(15)~~$-3x^2~+~29x~-40$

~~~~~~~~~$=-(3x^2~-29x~+~40)$

~~~~~~~~~$=-(3x-5)(x-8)$

(16)~~$-6x^2~+~8x~-2$

~~~~~~~~~$=-2(3x^2~-4x~+~1)$

~~~~~~~~~$=-2(x-1)(3x-1)$

(17)~~$-9x^2~-9x~+~54$

~~~~~~~~~$=-9(x^2~+~x~-6)$

~~~~~~~~~$=-9(x-2)(x+3)$

(18)~~$-12x^2~+~34x~-24$

~~~~~~~~~$=-2(6x^2~-17x~+~12)$

~~~~~~~~~$=-2(2x-3)(3x-4)$

(19)~~$16x^2~+~52x~+~42$

~~~~~~~~~$=2(8x^2~+~26x~+~21)$

~~~~~~~~~$=2(4x+7)(2x+3)$

(20)~~$-30x~+~70$

~~~~~~~~~$=-10(3x-7)$

(21)~~$12x^2~-5x~-72$

~~~~~~~~~$=(3x-8)(4x+9)$

(22)~~$-4x^2~-20x~+~56$

~~~~~~~~~$=-4(x^2~+~5x~-14)$

~~~~~~~~~$=-4(x+7)(x-2)$

(23)~~$-x^2~-3x$

~~~~~~~~~$=-x(x+3)$

(24)~~$3x^2~+~13x~-56$

~~~~~~~~~$=(x+7)(3x-8)$

(25)~~$-2x^2~+~5x~+~7$

~~~~~~~~~$=-(2x^2~-5x~-7)$

~~~~~~~~~$=-(x+1)(2x-7)$

\end{document}
