\documentclass[a4j,twocolumn,10pt,fleqn]{jarticle}
\usepackage[dvipdfmx]{graphicx}
% \usepackage[dvipdfmx]{color}
\usepackage{here}
\usepackage{longtable}
\usepackage{bm}
\usepackage{amsmath,amssymb}
\usepackage{float}
\usepackage{txfonts}
\usepackage{mathrsfs}
\usepackage{subcaption}
\usepackage{lscape}
\usepackage{textcomp}
\usepackage{multirow}
\usepackage{afterpage}
\usepackage{color}
\usepackage{tabularx}
\usepackage{pythontex}
\begin{document}
tip: $a(x - p)^2 + q$

~~~~~~~~~$= a(x^2 - 2px + p^2) + q$

~~~~~~~~~$= ax^2 - 2apx + ap^2 + q$

(1)~~$(x-3)^2 +4$

~~~~~~~~~$=x^2-6x +13$

(2)~~$-(x-10)^2-5$

~~~~~~~~~$=-(x^2-20x +100)-5$

~~~~~~~~~$=-x^2 +20x-105$

(3)~~$-2(x-10)^2 +4$

~~~~~~~~~$=-2(x^2-20x +100) +4$

~~~~~~~~~$=-2x^2 +40x-196$

(4)~~$2(x-5)^2 +4$

~~~~~~~~~$=2(x^2-10x +25) +4$

~~~~~~~~~$=2x^2-20x +54$

(5)~~$3(x +9)^2 +2$

~~~~~~~~~$=3(x^2 +18x +81) +2$

~~~~~~~~~$=3x^2 +54x +245$

(6)~~$-3(x +7)^2 +2$

~~~~~~~~~$=-3(x^2 +14x +49) +2$

~~~~~~~~~$=-3x^2-42x-145$

(7)~~$-2(x +3)^2-1$

~~~~~~~~~$=-2(x^2 +6x +9)-1$

~~~~~~~~~$=-2x^2-12x-19$

(8)~~$4(x-1)^2-5$

~~~~~~~~~$=4(x^2-2x +1)-5$

~~~~~~~~~$=4x^2-8x-1$

(9)~~$-(x-10)^2-5$

~~~~~~~~~$=-(x^2-20x +100)-5$

~~~~~~~~~$=-x^2 +20x-105$

(10)~~$-3(x-7)^2 +2$

~~~~~~~~~$=-3(x^2-14x +49) +2$

~~~~~~~~~$=-3x^2 +42x-145$

(11)~~$-3(x-1)^2 +4$

~~~~~~~~~$=-3(x^2-2x +1) +4$

~~~~~~~~~$=-3x^2 +6x +1$

(12)~~$4(x +1)^2-5$

~~~~~~~~~$=4(x^2 +2x +1)-5$

~~~~~~~~~$=4x^2 +8x-1$

(13)~~$-2(x-8)^2 +2$

~~~~~~~~~$=-2(x^2-16x +64) +2$

~~~~~~~~~$=-2x^2 +32x-126$

(14)~~$-2(x-5)^2-2$

~~~~~~~~~$=-2(x^2-10x +25)-2$

~~~~~~~~~$=-2x^2 +20x-52$

(15)~~$3(x-1)^2-3$

~~~~~~~~~$=3(x^2-2x +1)-3$

~~~~~~~~~$=3x^2-6x$

(16)~~$4(x-6)^2 +2$

~~~~~~~~~$=4(x^2-12x +36) +2$

~~~~~~~~~$=4x^2-48x +146$

(17)~~$-4(x-6)^2-3$

~~~~~~~~~$=-4(x^2-12x +36)-3$

~~~~~~~~~$=-4x^2 +48x-147$

(18)~~$(x-8)^2-2$

~~~~~~~~~$=x^2-16x +62$

(19)~~$(x-2)^2-1$

~~~~~~~~~$=x^2-4x +3$

(20)~~$-5(x-1)^2-1$

~~~~~~~~~$=-5(x^2-2x +1)-1$

~~~~~~~~~$=-5x^2 +10x-6$

(21)~~$-4(x-6)^2-1$

~~~~~~~~~$=-4(x^2-12x +36)-1$

~~~~~~~~~$=-4x^2 +48x-145$

(22)~~$-5(x-1)^2-2$

~~~~~~~~~$=-5(x^2-2x +1)-2$

~~~~~~~~~$=-5x^2 +10x-7$

(23)~~$-5(x-4)^2-4$

~~~~~~~~~$=-5(x^2-8x +16)-4$

~~~~~~~~~$=-5x^2 +40x-84$

(24)~~$3(x-5)^2-2$

~~~~~~~~~$=3(x^2-10x +25)-2$

~~~~~~~~~$=3x^2-30x +73$

(25)~~$4(x-7)^2-5$

~~~~~~~~~$=4(x^2-14x +49)-5$

~~~~~~~~~$=4x^2-56x +191$

\end{document}
