\documentclass[a4j,twocolumn,10pt,fleqn]{jarticle}
\usepackage[dvipdfmx]{graphicx}
% \usepackage[dvipdfmx]{color}
\usepackage{here}
\usepackage{longtable}
\usepackage{bm}
\usepackage{amsmath,amssymb}
\usepackage{float}
\usepackage{txfonts}
\usepackage{mathrsfs}
\usepackage{subcaption}
\usepackage{lscape}
\usepackage{textcomp}
\usepackage{multirow}
\usepackage{afterpage}
\usepackage{color}
\usepackage{tabularx}
\usepackage{pythontex}
\begin{document}
tip: $\left(a x + b\right) \left(a^{2} x^{2} - a b x + b^{2}\right)$

~~~~~~~~~$=a^{3} x^{3} + b^{3}$


(1)~~$\left(4 x - 1\right) \left(16 x^{2} + 4 x + 1\right)$

~~~~~~~~~$=64 x^{3} - 1$

(2)~~$\left(4 x + 7\right) \left(16 x^{2} - 28 x + 49\right)$

~~~~~~~~~$=64 x^{3} + 343$

(3)~~$\left(x + 1\right) \left(x^{2} - x + 1\right)$

~~~~~~~~~$=x^{3} + 1$

(4)~~$\left(5 x - 9\right) \left(25 x^{2} + 45 x + 81\right)$

~~~~~~~~~$=125 x^{3} - 729$

(5)~~$\left(5 x + 7\right) \left(25 x^{2} - 35 x + 49\right)$

~~~~~~~~~$=125 x^{3} + 343$

(6)~~$\left(x - 1\right) \left(x^{2} + x + 1\right)$

~~~~~~~~~$=x^{3} - 1$

(7)~~$\left(x + 2\right) \left(x^{2} - 2 x + 4\right)$

~~~~~~~~~$=x^{3} + 8$

(8)~~$\left(2 x + 9\right) \left(4 x^{2} - 18 x + 81\right)$

~~~~~~~~~$=8 x^{3} + 729$

(9)~~$\left(3 x - 8\right) \left(9 x^{2} + 24 x + 64\right)$

~~~~~~~~~$=27 x^{3} - 512$

(10)~~$\left(x + 5\right) \left(x^{2} - 5 x + 25\right)$

~~~~~~~~~$=x^{3} + 125$

(11)~~$\left(4 x + 1\right) \left(16 x^{2} - 4 x + 1\right)$

~~~~~~~~~$=64 x^{3} + 1$

(12)~~$\left(x + 2\right) \left(x^{2} - 2 x + 4\right)$

~~~~~~~~~$=x^{3} + 8$

(13)~~$\left(2 x + 9\right) \left(4 x^{2} - 18 x + 81\right)$

~~~~~~~~~$=8 x^{3} + 729$

(14)~~$\left(x - 3\right) \left(x^{2} + 3 x + 9\right)$

~~~~~~~~~$=x^{3} - 27$

(15)~~$\left(x - 3\right) \left(x^{2} + 3 x + 9\right)$

~~~~~~~~~$=x^{3} - 27$

(16)~~$\left(2 x + 7\right) \left(4 x^{2} - 14 x + 49\right)$

~~~~~~~~~$=8 x^{3} + 343$

(17)~~$\left(x + 9\right) \left(x^{2} - 9 x + 81\right)$

~~~~~~~~~$=x^{3} + 729$

(18)~~$\left(3 x - 8\right) \left(9 x^{2} + 24 x + 64\right)$

~~~~~~~~~$=27 x^{3} - 512$

(19)~~$\left(3 x - 4\right) \left(9 x^{2} + 12 x + 16\right)$

~~~~~~~~~$=27 x^{3} - 64$

(20)~~$\left(2 x - 7\right) \left(4 x^{2} + 14 x + 49\right)$

~~~~~~~~~$=8 x^{3} - 343$

(21)~~$\left(4 x - 9\right) \left(16 x^{2} + 36 x + 81\right)$

~~~~~~~~~$=64 x^{3} - 729$

(22)~~$\left(x + 3\right) \left(x^{2} - 3 x + 9\right)$

~~~~~~~~~$=x^{3} + 27$

(23)~~$\left(3 x + 2\right) \left(9 x^{2} - 6 x + 4\right)$

~~~~~~~~~$=27 x^{3} + 8$

(24)~~$\left(2 x - 1\right) \left(4 x^{2} + 2 x + 1\right)$

~~~~~~~~~$=8 x^{3} - 1$

(25)~~$\left(x - 6\right) \left(x^{2} + 6 x + 36\right)$

~~~~~~~~~$=x^{3} - 216$

(26)~~$\left(3 x - 7\right) \left(9 x^{2} + 21 x + 49\right)$

~~~~~~~~~$=27 x^{3} - 343$

(27)~~$\left(2 x + 3\right) \left(4 x^{2} - 6 x + 9\right)$

~~~~~~~~~$=8 x^{3} + 27$

(28)~~$\left(4 x - 3\right) \left(16 x^{2} + 12 x + 9\right)$

~~~~~~~~~$=64 x^{3} - 27$

(29)~~$\left(5 x + 3\right) \left(25 x^{2} - 15 x + 9\right)$

~~~~~~~~~$=125 x^{3} + 27$

(30)~~$\left(3 x - 4\right) \left(9 x^{2} + 12 x + 16\right)$

~~~~~~~~~$=27 x^{3} - 64$

(31)~~$\left(2 x - 1\right) \left(4 x^{2} + 2 x + 1\right)$

~~~~~~~~~$=8 x^{3} - 1$

(32)~~$\left(2 x - 5\right) \left(4 x^{2} + 10 x + 25\right)$

~~~~~~~~~$=8 x^{3} - 125$

(33)~~$\left(x + 3\right) \left(x^{2} - 3 x + 9\right)$

~~~~~~~~~$=x^{3} + 27$

(34)~~$\left(2 x + 3\right) \left(4 x^{2} - 6 x + 9\right)$

~~~~~~~~~$=8 x^{3} + 27$

(35)~~$\left(x - 1\right) \left(x^{2} + x + 1\right)$

~~~~~~~~~$=x^{3} - 1$

(36)~~$\left(x - 8\right) \left(x^{2} + 8 x + 64\right)$

~~~~~~~~~$=x^{3} - 512$

(37)~~$\left(2 x + 5\right) \left(4 x^{2} - 10 x + 25\right)$

~~~~~~~~~$=8 x^{3} + 125$

(38)~~$\left(5 x + 1\right) \left(25 x^{2} - 5 x + 1\right)$

~~~~~~~~~$=125 x^{3} + 1$

(39)~~$\left(x + 1\right) \left(x^{2} - x + 1\right)$

~~~~~~~~~$=x^{3} + 1$

(40)~~$\left(x + 6\right) \left(x^{2} - 6 x + 36\right)$

~~~~~~~~~$=x^{3} + 216$

(41)~~$\left(3 x + 7\right) \left(9 x^{2} - 21 x + 49\right)$

~~~~~~~~~$=27 x^{3} + 343$

(42)~~$\left(4 x + 7\right) \left(16 x^{2} - 28 x + 49\right)$

~~~~~~~~~$=64 x^{3} + 343$

(43)~~$\left(x + 5\right) \left(x^{2} - 5 x + 25\right)$

~~~~~~~~~$=x^{3} + 125$

(44)~~$\left(4 x + 9\right) \left(16 x^{2} - 36 x + 81\right)$

~~~~~~~~~$=64 x^{3} + 729$

(45)~~$\left(5 x - 7\right) \left(25 x^{2} + 35 x + 49\right)$

~~~~~~~~~$=125 x^{3} - 343$

(46)~~$\left(x + 1\right) \left(x^{2} - x + 1\right)$

~~~~~~~~~$=x^{3} + 1$

(47)~~$\left(3 x - 1\right) \left(9 x^{2} + 3 x + 1\right)$

~~~~~~~~~$=27 x^{3} - 1$

(48)~~$\left(2 x + 1\right) \left(4 x^{2} - 2 x + 1\right)$

~~~~~~~~~$=8 x^{3} + 1$

(49)~~$\left(x + 1\right) \left(x^{2} - x + 1\right)$

~~~~~~~~~$=x^{3} + 1$

(50)~~$\left(2 x - 3\right) \left(4 x^{2} + 6 x + 9\right)$

~~~~~~~~~$=8 x^{3} - 27$

\end{document}
