\documentclass[a4j,twocolumn,10pt,fleqn]{jarticle}
\usepackage[dvipdfmx]{graphicx}
% \usepackage[dvipdfmx]{color}
\usepackage{here}
\usepackage{longtable}
\usepackage{bm}
\usepackage{amsmath,amssymb}
\usepackage{float}
\usepackage{txfonts}
\usepackage{mathrsfs}
\usepackage{subcaption}
\usepackage{lscape}
\usepackage{textcomp}
\usepackage{multirow}
\usepackage{afterpage}
\usepackage{color}
\usepackage{tabularx}
\usepackage{pythontex}
\begin{document}
tip: $P(ax + b)(cx + d) = Pacx^2 + P(ad + bc)x + Pbd$

(1)~~$6(x-5)$

~~~~~~~~~$=6x~-30$

(2)~~$-(x-6)(x+7)$

~~~~~~~~~$=-x^2~-x~+~42$

(3)~~$2(x+2)(3x-4)$

~~~~~~~~~$=6x^2~+~4x~-16$

(4)~~$-(2x-5)(3x+2)$

~~~~~~~~~$=-6x^2~+~11x~+~10$

(5)~~$-(x-8)(4x+7)$

~~~~~~~~~$=-4x^2~+~25x~+~56$

(6)~~$-2(x-6)(x+1)$

~~~~~~~~~$=-2x^2~+~10x~+~12$

(7)~~$(4x+7)(2x+9)$

~~~~~~~~~$=8x^2~+~50x~+~63$

(8)~~$-9(3x+7)$

~~~~~~~~~$=-27x~-63$

(9)~~$4(x+1)(5x-7)$

~~~~~~~~~$=20x^2~-8x~-28$

(10)~~$-2(x+1)(x-1)$

~~~~~~~~~$=-2x^2~+~2$

(11)~~$-2(2x+3)(x-4)$

~~~~~~~~~$=-4x^2~+~10x~+~24$

(12)~~$4(2x+5)(x+1)$

~~~~~~~~~$=8x^2~+~28x~+~20$

(13)~~$-7(2x+7)$

~~~~~~~~~$=-14x~-49$

(14)~~$-(x-1)(3x+2)$

~~~~~~~~~$=-3x^2~+~x~+~2$

(15)~~$6(x+2)(x-2)$

~~~~~~~~~$=6x^2~-24$

(16)~~$3(x-3)(3x+8)$

~~~~~~~~~$=9x^2~-3x~-72$

(17)~~$-2(2x+1)(3x-7)$

~~~~~~~~~$=-12x^2~+~22x~+~14$

(18)~~$-2(4x-3)(x-1)$

~~~~~~~~~$=-8x^2~+~14x~-6$

(19)~~$-4(3x+4)(x-1)$

~~~~~~~~~$=-12x^2~-4x~+~16$

(20)~~$-27(x-1)$

~~~~~~~~~$=-27x~+~27$

(21)~~$4(5x-2)(x-1)$

~~~~~~~~~$=20x^2~-28x~+~8$

(22)~~$-6(x-3)^2$

~~~~~~~~~$=-6x^2~+~36x~-54$

(23)~~$(5x-2)(5x+8)$

~~~~~~~~~$=25x^2~+~30x~-16$

(24)~~$-2(x+3)(x-3)$

~~~~~~~~~$=-2x^2~+~18$

(25)~~$-(4x+5)(x-1)$

~~~~~~~~~$=-4x^2~-x~+~5$

(26)~~$-2(x+4)(x+5)$

~~~~~~~~~$=-2x^2~-18x~-40$

(27)~~$-10(x+2)(x+1)$

~~~~~~~~~$=-10x^2~-30x~-20$

(28)~~$-(5x-7)(3x-7)$

~~~~~~~~~$=-15x^2~+~56x~-49$

(29)~~$-6(x+1)(x+2)$

~~~~~~~~~$=-6x^2~-18x~-12$

(30)~~$-2(2x-1)(x+3)$

~~~~~~~~~$=-4x^2~-10x~+~6$

(31)~~$10(x-2)(x+2)$

~~~~~~~~~$=10x^2~-40$

(32)~~$4x(x+2)$

~~~~~~~~~$=4x^2~+~8x$

(33)~~$-(4x-1)(3x+1)$

~~~~~~~~~$=-12x^2~-x~+~1$

(34)~~$-2(2x+1)(5x-4)$

~~~~~~~~~$=-20x^2~+~6x~+~8$

(35)~~$2(2x-3)(x-3)$

~~~~~~~~~$=4x^2~-18x~+~18$

(36)~~$-(4x-7)(x-5)$

~~~~~~~~~$=-4x^2~+~27x~-35$

(37)~~$-9(2x+9)$

~~~~~~~~~$=-18x~-81$

(38)~~$-(5x+1)(x+4)$

~~~~~~~~~$=-5x^2~-21x~-4$

(39)~~$(x-9)(3x+2)$

~~~~~~~~~$=3x^2~-25x~-18$

(40)~~$(x+8)(x-1)$

~~~~~~~~~$=x^2~+~7x~-8$

(41)~~$-(4x-9)(x-7)$

~~~~~~~~~$=-4x^2~+~37x~-63$

(42)~~$-3(x-3)(x-2)$

~~~~~~~~~$=-3x^2~+~15x~-18$

(43)~~$-(2x-3)(4x+7)$

~~~~~~~~~$=-8x^2~-2x~+~21$

(44)~~$4(x-5)(x+1)$

~~~~~~~~~$=4x^2~-16x~-20$

(45)~~$-2(2x-1)^2$

~~~~~~~~~$=-8x^2~+~8x~-2$

(46)~~$2(x-3)(x-6)$

~~~~~~~~~$=2x^2~-18x~+~36$

(47)~~$(5x+4)(4x-1)$

~~~~~~~~~$=20x^2~+~11x~-4$

(48)~~$-2(2x+1)(3x-2)$

~~~~~~~~~$=-12x^2~+~2x~+~4$

(49)~~$-(2x+5)(4x-7)$

~~~~~~~~~$=-8x^2~-6x~+~35$

(50)~~$(4x+3)(5x-9)$

~~~~~~~~~$=20x^2~-21x~-27$

(51)~~$(x+9)(3x-8)$

~~~~~~~~~$=3x^2~+~19x~-72$

(52)~~$-(x-6)(4x+7)$

~~~~~~~~~$=-4x^2~+~17x~+~42$

(53)~~$-2(3x+8)(x+5)$

~~~~~~~~~$=-6x^2~-46x~-80$

(54)~~$2(3x-1)(x+3)$

~~~~~~~~~$=6x^2~+~16x~-6$

(55)~~$2(x+7)(2x-1)$

~~~~~~~~~$=4x^2~+~26x~-14$

(56)~~$(5x+1)(x+9)$

~~~~~~~~~$=5x^2~+~46x~+~9$

(57)~~$3(x+2)(3x+4)$

~~~~~~~~~$=9x^2~+~30x~+~24$

(58)~~$-(3x-2)(4x+7)$

~~~~~~~~~$=-12x^2~-13x~+~14$

(59)~~$3(x-4)$

~~~~~~~~~$=3x~-12$

(60)~~$4(x-1)(2x+9)$

~~~~~~~~~$=8x^2~+~28x~-36$

(61)~~$-3(4x-7)(x-3)$

~~~~~~~~~$=-12x^2~+~57x~-63$

(62)~~$4(x-1)(x-4)$

~~~~~~~~~$=4x^2~-20x~+~16$

(63)~~$-(3x+5)(3x-4)$

~~~~~~~~~$=-9x^2~-3x~+~20$

(64)~~$-3(5x-7)(x-2)$

~~~~~~~~~$=-15x^2~+~51x~-42$

(65)~~$-(x-5)(2x-3)$

~~~~~~~~~$=-2x^2~+~13x~-15$

(66)~~$6(x+2)(x+3)$

~~~~~~~~~$=6x^2~+~30x~+~36$

(67)~~$-(2x-7)(4x-5)$

~~~~~~~~~$=-8x^2~+~38x~-35$

(68)~~$-(2x+3)(2x-3)$

~~~~~~~~~$=-4x^2~+~9$

(69)~~$-2(2x+1)(3x+2)$

~~~~~~~~~$=-12x^2~-14x~-4$

(70)~~$3(x-1)(x-6)$

~~~~~~~~~$=3x^2~-21x~+~18$

(71)~~$(4x-3)(3x+4)$

~~~~~~~~~$=12x^2~+~7x~-12$

(72)~~$(3x-8)(x+4)$

~~~~~~~~~$=3x^2~+~4x~-32$

(73)~~$2(x+9)(x-3)$

~~~~~~~~~$=2x^2~+~12x~-54$

(74)~~$-(4x-1)(3x-5)$

~~~~~~~~~$=-12x^2~+~23x~-5$

(75)~~$-3(3x+4)(x-2)$

~~~~~~~~~$=-9x^2~+~6x~+~24$

(76)~~$3(x+2)(x+9)$

~~~~~~~~~$=3x^2~+~33x~+~54$

(77)~~$4(x+3)(x-3)$

~~~~~~~~~$=4x^2~-36$

(78)~~$-2(4x+7)$

~~~~~~~~~$=-8x~-14$

(79)~~$-3(x+8)$

~~~~~~~~~$=-3x~-24$

(80)~~$5(5x+6)(x+2)$

~~~~~~~~~$=25x^2~+~80x~+~60$

(81)~~$3(x-3)(5x+4)$

~~~~~~~~~$=15x^2~-33x~-36$

(82)~~$2(3x+8)$

~~~~~~~~~$=6x~+~16$

(83)~~$2(2x+3)(x+9)$

~~~~~~~~~$=4x^2~+~42x~+~54$

(84)~~$(5x-6)(x+10)$

~~~~~~~~~$=5x^2~+~44x~-60$

(85)~~$7(2x-5)$

~~~~~~~~~$=14x~-35$

(86)~~$(x-7)(3x-2)$

~~~~~~~~~$=3x^2~-23x~+~14$

(87)~~$(x-10)(2x+1)$

~~~~~~~~~$=2x^2~-19x~-10$

(88)~~$-(x+3)(5x+3)$

~~~~~~~~~$=-5x^2~-18x~-9$

(89)~~$-8(x-4)(x+1)$

~~~~~~~~~$=-8x^2~+~24x~+~32$

(90)~~$(x+9)(2x-3)$

~~~~~~~~~$=2x^2~+~15x~-27$

(91)~~$-(2x-5)(x+10)$

~~~~~~~~~$=-2x^2~-15x~+~50$

(92)~~$-(x+1)(5x-4)$

~~~~~~~~~$=-5x^2~-x~+~4$

(93)~~$2(x-2)(x-4)$

~~~~~~~~~$=2x^2~-12x~+~16$

(94)~~$(5x+3)(x-1)$

~~~~~~~~~$=5x^2~-2x~-3$

(95)~~$4(x-2)(2x+5)$

~~~~~~~~~$=8x^2~+~4x~-40$

(96)~~$8(5x-6)$

~~~~~~~~~$=40x~-48$

(97)~~$(4x+7)(5x+7)$

~~~~~~~~~$=20x^2~+~63x~+~49$

(98)~~$-(2x-7)(2x+1)$

~~~~~~~~~$=-4x^2~+~12x~+~7$

(99)~~$-3(x+2)(x+5)$

~~~~~~~~~$=-3x^2~-21x~-30$

(100)~~$(5x-1)(x+1)$

~~~~~~~~~$=5x^2~+~4x~-1$

\end{document}
