\documentclass[a4j,twocolumn,10pt,fleqn]{jarticle}
\usepackage[dvipdfmx]{graphicx}
% \usepackage[dvipdfmx]{color}
\usepackage{here}
\usepackage{longtable}
\usepackage{bm}
\usepackage{amsmath,amssymb}
\usepackage{float}
\usepackage{txfonts}
\usepackage{mathrsfs}
\usepackage{subcaption}
\usepackage{lscape}
\usepackage{textcomp}
\usepackage{multirow}
\usepackage{afterpage}
\usepackage{color}
\usepackage{tabularx}
\usepackage{pythontex}
\begin{document}
tip:~~$Pacx^2 + P(ad + bc)x + Pbd$

~~~~~~~~~$= P\{acx^2 + (ad + bc)x +bd\}$

~~~~~~~~~$= P(ax + b)(cx + d)$

(1)~~$9x^2~-6x$

~~~~~~~~~$=3x(3x-2)$

(2)~~$-2x^2~+~9x~+~5$

~~~~~~~~~$=-(2x^2~-9x~-5)$

~~~~~~~~~$=-(2x+1)(x-5)$

(3)~~$-2x^2~-19x~-35$

~~~~~~~~~$=-(2x^2~+~19x~+~35)$

~~~~~~~~~$=-(x+7)(2x+5)$

(4)~~$-5x^2~-36x~+~81$

~~~~~~~~~$=-(5x^2~+~36x~-81)$

~~~~~~~~~$=-(x+9)(5x-9)$

(5)~~$35x~-7$

~~~~~~~~~$=7(5x-1)$

(6)~~$-4x^2~-12x~-8$

~~~~~~~~~$=-4(x^2~+~3x~+~2)$

~~~~~~~~~$=-4(x+2)(x+1)$

(7)~~$2x^2~-8x~-24$

~~~~~~~~~$=2(x^2~-4x~-12)$

~~~~~~~~~$=2(x+2)(x-6)$

(8)~~$-2x^2~-2x~+~12$

~~~~~~~~~$=-2(x^2~+~x~-6)$

~~~~~~~~~$=-2(x-2)(x+3)$

(9)~~$-3x^2~-9x~-6$

~~~~~~~~~$=-3(x^2~+~3x~+~2)$

~~~~~~~~~$=-3(x+1)(x+2)$

(10)~~$-6x^2~+~42x~-72$

~~~~~~~~~$=-6(x^2~-7x~+~12)$

~~~~~~~~~$=-6(x-4)(x-3)$

(11)~~$15x^2~+~64x~+~64$

~~~~~~~~~$=(3x+8)(5x+8)$

(12)~~$4x^2~+~28x~+~48$

~~~~~~~~~$=4(x^2~+~7x~+~12)$

~~~~~~~~~$=4(x+4)(x+3)$

(13)~~$3x^2~-25x~+~8$

~~~~~~~~~$=(3x-1)(x-8)$

(14)~~$-8x~-4$

~~~~~~~~~$=-4(2x+1)$

(15)~~$-3x^2~-19x~-30$

~~~~~~~~~$=-(3x^2~+~19x~+~30)$

~~~~~~~~~$=-(3x+10)(x+3)$

(16)~~$-3x^2~+~12x~-9$

~~~~~~~~~$=-3(x^2~-4x~+~3)$

~~~~~~~~~$=-3(x-3)(x-1)$

(17)~~$-8x^2~-48x~-70$

~~~~~~~~~$=-2(4x^2~+~24x~+~35)$

~~~~~~~~~$=-2(2x+7)(2x+5)$

(18)~~$4x^2~+~33x~-70$

~~~~~~~~~$=(x+10)(4x-7)$

(19)~~$6x^2~-11x~+~3$

~~~~~~~~~$=(3x-1)(2x-3)$

(20)~~$-10x^2~+~22x~-12$

~~~~~~~~~$=-2(5x^2~-11x~+~6)$

~~~~~~~~~$=-2(5x-6)(x-1)$

(21)~~$6x^2~-29x~+~30$

~~~~~~~~~$=(3x-10)(2x-3)$

(22)~~$25x^2~-30x~+~8$

~~~~~~~~~$=(5x-2)(5x-4)$

(23)~~$20x^2~+~37x~+~8$

~~~~~~~~~$=(4x+1)(5x+8)$

(24)~~$-15x^2~+~46x~-16$

~~~~~~~~~$=-(15x^2~-46x~+~16)$

~~~~~~~~~$=-(5x-2)(3x-8)$

(25)~~$8x^2~-8x~-16$

~~~~~~~~~$=8(x^2~-x~-2)$

~~~~~~~~~$=8(x-2)(x+1)$

\end{document}
